developed rewrite principles for calling interp_mtree on the variable it is targetting

theories/AlmostStlc/Examples.v
@@ -27,30 +27,17 @@ Context {Γ : ctx}.
 
 Definition plus_call : call_frame := [(Nat, Arrow Nat [] Nat)].
 
-Definition plus : term (Arrow Nat [] (Arrow Nat [] Nat)) Γ [].
-apply term_abs. apply term_abs.
-apply @term_mfix with (R := plus_call) (MR := [plus_call]) (x := VarZ).
-- apply mfix_bodies_cons.
-  + eapply term_match_nat.
-    * apply term_var. apply VarZ.
-    * apply term_abs. apply term_var. apply VarZ.
-    * eapply @term_app with (t1 := Arrow Nat [] Nat).
-      {
-        apply term_abs. apply term_abs.
-        apply @term_app with (t1 := Nat).
-        - exact (term_var (VarS VarZ)).
-        - exact (term_succ (term_var VarZ)).
-      }
-      {
-        exact (term_call VarZ VarZ (term_var VarZ)).
-      }
-  + apply mfix_bodies_nil.
-- eapply @term_app with (t1 := Nat).
-  + apply @term_app with (t1 := Arrow Nat [] Nat).
-    * apply @fun_lift with (MR1 := [plus_call]).
-    * exact (term_call VarZ VarZ (term_var VarZ)).
-  + exact (term_var (VarS VarZ)). 
-Defined.
+Definition plus : term (Arrow Nat [] (Arrow Nat [] Nat)) Γ [] :=
+term_abs
+  (term_abs
+     (term_mfix plus_call VarZ
+        (mfix_bodies_cons
+           (term_match_nat (term_var VarZ) (term_abs (term_var VarZ))
+              (term_app
+                 (term_abs (term_abs (term_app (term_var (VarS VarZ)) (term_succ (term_var VarZ)))))
+                 (term_call VarZ VarZ (term_var VarZ)))) mfix_bodies_nil)
+        (term_app (term_app (@fun_lift _ [plus_call] _ _ _ _) 
+                            (term_call VarZ VarZ (term_var VarZ))) (term_var (VarS VarZ))))).
 
 End plus.
 
@@ -60,35 +47,70 @@ Context {Γ : ctx} {MR : mfix_ctx}.
 
 Definition plus_call' : call_frame := [(Pair Nat Nat, Nat) ].
 
-Definition plus' : term (Arrow (Pair Nat Nat) MR Nat) Γ MR.
-apply term_abs. 
-eapply @term_mfix with (R := plus_call') (MR := plus_call' :: MR) (x := VarZ).
-- apply mfix_bodies_cons.
-  + eapply term_split.
-    * apply term_var. apply VarZ.
-    * eapply term_match_nat.
-      -- eapply term_var. eapply VarZ.
-      -- eapply term_var. eapply VarS. eapply VarZ.
-      -- apply term_succ. eapply term_call.
-         apply VarZ. apply VarZ.
-         apply term_pair.
-         apply term_var. apply VarZ.
-         apply term_var. apply VarS. apply VarS. apply VarZ.
-  + apply mfix_bodies_nil.
-- eapply term_call. apply VarZ. apply VarZ.
-  apply term_var. apply VarZ.
-Defined.
+Definition plus' : term (Arrow (Pair Nat Nat) MR Nat) Γ MR :=
+term_abs
+  (term_mfix plus_call' VarZ
+     (mfix_bodies_cons
+        (term_split (term_var VarZ)
+           (term_match_nat (term_var VarZ) (term_var (VarS VarZ))
+              (term_succ
+                 (term_call VarZ VarZ (term_pair (term_var VarZ) (term_var (VarS (VarS VarZ))))))))
+        mfix_bodies_nil) (term_call VarZ VarZ (term_var VarZ))).
+
 End plus'.
 
 Locate bind_ret_l.
 
+Require Import Paco.paco.
+
 Goal denote_term (term_app (@plus' [] []) (term_pair (term_const 1) (term_const 1))) tt ≈ 
        Ret 2.
+simp denote_term. repeat setoid_rewrite bind_bind. 
+unfold plus'. simp denote_term. do 4 setoid_rewrite bind_ret_l. 
+simp term_call. simp denote_term. simp denote_mfix_ctx. unfold plus_call'.
+simp denote_var.
+match goal with |- mapE ?h (interp_mtree ?MR ?R ?t ?x ?f ?m) ≈ _ => 
+                  idtac MR;
+                  idtac R;
+                  idtac t;
+                  idtac x;
+                  idtac f;
+                  idtac m
+end.
+(*next thing to do is *)
+s
+unfold plus
+simp denote_call_frame. setoid_rewrite bind_ret_l.
+
+setoid_rewrite bind_ret_l.
+setoid_rewrite bind_ret_l.
+unfold Monad.ret. cbn. 
+simp index_ctx.
+
+ setoid_rewrite index_ctx_equation_1.
+setoid_rewrite bind_ret_l.
+setoid_rewrite bind_ret_l.
+ unfold Monad.ret. cbn. 
+unfold plus'. simp denote_term. unfold Monad.ret. cbn. 
+match goal with |- EnTree.bind (Ret ?x) ?k ≈ Ret 2 => specialize (bind_ret_l x k) as H end.
+cbn in H. apply eq_sub_eutt in H.
+Print Instances Proper.
+ csetoid_rewrite bind_ret_l in H. (*don't see why this rewrite is not working *) setoid_rewrite H at 1.
+(* might need more properness*)
+setoid_rewrite bind_ret_l.
+ setoid_rewrite bind_ret_l at 2.
+setoid_rewrite bind_ret_l.
+pstep. red. cbn. simp denote_term. cbn. unfold plus'. simp denote_term.
+cbn. unfold observe at 1. unfold EnTree.bind, EnTree.subst, EnTree.subst'.  cbn. cbn. cbn. red.
 simp denote_term. unfold plus'. simp denote_term. 
 repeat setoid_rewrite bind_ret_l. unfold plus_call'. simp denote_term.
-cbn. simp denote_term. Transparent denote_term. cbn.
+simp remove_denote. 
+cbn. simp denote_term. pstep. Transparent denote_term. unfold mapE. cbn. unfold mapE'. cbn.
+repeat simp denote_mrec_ctx. simp remove. setoid_rewrite denote_var_equation_1. simp denote_var.
+ pfold.
 (* setoid_rewrite bind_ret_l.
  unfold denote_term.  setoid_rewrite @denote_term_equation_15. *)
+Abort.
 Section map_term.
 Context (t1 t2 : type) (MR : mfix_ctx).
 
@@ -96,33 +118,20 @@ Definition map_call : call_frame := (List t1, List t2) :: nil.
 
 
 (* should come up with some notations and   *)
-Definition map_body : term (List t2) (List t1 :: List t1 :: (Arrow t1 MR t2 :: nil))%list (map_call :: MR).
-eapply term_match_list.
-- eapply term_var. eapply VarS. eapply VarZ.
-- eapply term_nil.
-- eapply term_cons.
-  + eapply term_lift with (MR1 := [map_call]).
-    eapply term_app.
-    * eapply term_var. repeat constructor.
-    * eapply term_var. constructor.
-  + eapply term_call.
-    * apply VarZ.
-    * apply VarZ.
-    * eapply term_var. apply VarS. apply VarZ.
-Defined.
+Definition map_body : term (List t2) (List t1 :: List t1 :: (Arrow t1 MR t2 :: nil))%list (map_call :: MR)
+                           :=
+term_match_list (term_var (VarS VarZ)) term_nil
+  (term_cons
+     (term_lift [map_call] (term_app (term_var (VarS (VarS (VarS (VarS VarZ))))) (term_var VarZ)))
+     (term_call VarZ VarZ (term_var (VarS VarZ)))).
 
 
-Definition map : term (Arrow (Arrow t1 MR t2) [] (Arrow (List t1) MR (List t2))) [] [].
-eapply term_abs. eapply term_abs.
-apply @term_mfix with (R := map_call) (MR := map_call :: MR) (x := VarZ).
-- apply mfix_bodies_cons.
-  + apply map_body.
-  + apply mfix_bodies_nil.
-- eapply term_call.
-  + apply VarZ.
-  + apply VarZ.
-  + eapply term_var. eapply VarZ.
-Defined.
+Definition map : term (Arrow (Arrow t1 MR t2) [] (Arrow (List t1) MR (List t2))) [] [] :=
+term_abs
+  (term_abs
+     (term_mfix map_call VarZ (mfix_bodies_cons map_body mfix_bodies_nil)
+        (term_call VarZ VarZ (term_var VarZ)))).
+
 End map_term.
 
 Goal False.
