theories/AlmostStlc/InterpMTreeFacts.v
@@ -1,0 +1,201 @@
+From Coq Require Import
+     Program
+     Setoid
+     Morphisms
+     Relations
+     Logic.FunctionalExtensionality
+.
+
+From Paco Require Import paco.
+
+From ITree Require Import
+     Basics.Basics
+     Basics.Monad
+     Basics.Tacs
+     Basics.HeterogeneousRelations
+     Eq.Paco2.
+
+From EnTree Require Import
+     Basics.HeterogeneousRelations
+     Core.EnTreeDefinition
+     Core.SubEvent
+     Eq.Eqit
+.
+
+Require Import ExtLib.Structures.Functor.
+Require Import ExtLib.Structures.Applicative.
+Require Import ExtLib.Structures.Monad.
+Require Import Program.Tactics.
+
+Require Import ITree.Basics.Basics.
+
+Require Export TypedVar MrecMonad.
+
+From Equations Require Import Equations Signature.
+
+
+Section interp_mtree_match.
+Context (MR : mrec_ctx) (In : Type) (Out : EncodedType In) (x : var (In && Out) MR).
+Context (body : forall i : In, mtree MR (encodes i)).
+
+Lemma interp_mtree_ret (R : Type) (r : R) : interp_mtree MR In Out x body (ret r) ≅ ret r.
+Proof. 
+  pstep. red. cbn. constructor. auto.
+Qed.
+
+Lemma interp_mtree_tau (R : Type) (m : mtree MR R) : interp_mtree MR In Out x body (Tau m) ≅
+                                                                 Tau (interp_mtree MR In Out x body m).
+Proof.
+  pstep. red. cbn. constructor. left. apply Reflexive_eqit. auto.
+Qed.
+
+Lemma observe_interp_mtree_vis R e (k : _ -> mtree MR R) :
+  observe (interp_mtree MR In Out x body (Vis e k)) =
+               match bring_to_front MR x e with
+               | inl i && f => TauF (interp_mtree MR In Out x body ((EnTree.bind (body i) (fun x => k (f x)) )))
+               | inr e' && f => VisF e' (fun x0 : encodes e' => interp_mtree MR In Out x body ((k (f x0))))
+               end.
+Proof.
+  destruct (bring_to_front MR x e)  eqn : Heq.
+  destruct x0; simpl; setoid_rewrite Heq; auto.
+Qed.
+
+Lemma interp_mtree_vis R e (k : _ -> mtree MR R) :
+  interp_mtree MR In Out x body (Vis e k) ≅
+               match bring_to_front MR x e with
+               | inl i && f  => Tau (interp_mtree MR In Out x body ((EnTree.bind (body i) (fun x => k (f x)))))
+               | inr e' && f => Vis e' (fun x0 : encodes e' => interp_mtree MR In Out x body ((k (f x0))))
+               end.
+Proof.
+  specialize (observe_interp_mtree_vis R e k) as H. symmetry in  H. apply simpobs in H.
+  rewrite <- H.
+  destruct (bring_to_front MR x e); destruct x0; reflexivity. 
+Qed.
+      
+End interp_mtree_match.
+
+Section interp_mtree_proper.
+
+Context (MR : mrec_ctx) (In : Type) (Out : EncodedType In) (x : var (In && Out) MR).
+Context (body1 body2 : forall i : In, mtree MR (encodes i)).
+Context (b1 b2 : bool).
+Context (Hbody : forall i, eqit eq b1 b2 (body1 i) (body2 i)).
+
+Theorem interp_mtree_proper  (R : Type): forall (m1 m2 : mtree MR R),
+  eqit eq b1 b2 m1 m2 -> eqit eq b1 b2 (interp_mtree MR In Out x body1 m1) (interp_mtree MR In Out x body2 m2).
+Proof.
+  ginit. gcofix CIH. intros m1 m2 Hm12.
+  punfold Hm12.
+  red in Hm12. genobs m1 om1. genobs m2 om2. 
+  hinduction Hm12 before r; intros; subst; pclearbot.
+  - gstep. red. unfold observe. simpl. setoid_rewrite <- Heqom1. setoid_rewrite <- Heqom2.
+    constructor. auto.
+  - gstep. red. unfold observe. simpl. setoid_rewrite <- Heqom1. setoid_rewrite <- Heqom2.
+    constructor. gfinal. left. eauto.
+  - unfold interp_mtree. rewrite <- Heqom1. rewrite <- Heqom2. 
+    gstep. red. setoid_rewrite observe_interp_mtree_vis. 
+    destruct (bring_to_front MR x e). destruct x0.
+    + constructor. gfinal. left. eapply CIH. eapply eqit_bind. apply Hbody.
+      intros. subst. apply REL.
+    + constructor. gfinal. left. eapply CIH. apply REL.
+  - unfold interp_mtree at 1. rewrite <- Heqom1. setoid_rewrite interp_mtree_tau.
+    inv CHECK. destruct b2;
+    rewrite tau_euttge; eauto. 
+  - unfold interp_mtree at 2. rewrite <- Heqom2. setoid_rewrite interp_mtree_tau.
+    inv CHECK. destruct b1; rewrite tau_euttge; eauto.
+Qed.
+
+End interp_mtree_proper.
+
+
+
+Definition ptwise {A : Type} {B : A -> Type} : (forall (a : A), relation (B a)) -> relation (forall (a : A), B a) :=
+  fun R (f g : forall a, B a) => forall a, (R a (f a) (g a) ).
+
+#[global] Instance interp_mtree_proper_inst R (MR : mrec_ctx) (In : Type) (Out : EncodedType In) (x : var (In && Out) MR) (b1 b2 : bool) :
+  Proper (ptwise (fun i => eqit (@eq (encodes i)) b1 b2 ) ==> eqit eq b1 b2 ==> eqit (@eq R) b1 b2 ) (@interp_mtree MR In Out x R).
+Proof.
+  repeat intro. eapply interp_mtree_proper; eauto.
+Qed.
+
+#[global] Instance interp_mtree_proper_inst' R (MR : mrec_ctx) (In : Type) (Out : EncodedType In) (x : var (In && Out) MR) (b1 b2 : bool) :
+  Proper (eq ==> eqit eq b1 b2 ==> eqit (@eq R) b1 b2 ) (@interp_mtree MR In Out x R).
+Proof.
+  repeat intro. eapply interp_mtree_proper; eauto. subst. intros. reflexivity.
+Qed.
+
+Section interp_mtree_bind.
+Context (MR : mrec_ctx) (In : Type) (Out : EncodedType In) (x : var (In && Out) MR).
+Context (body : forall i : In, mtree MR (encodes i)).
+
+Lemma interp_mtree_bind (R S : Type) (m : mtree _ R) (k : R -> mtree _ S) : 
+  interp_mtree MR In Out x body (bind m k) ≅
+               bind (interp_mtree MR In Out x body m) 
+               (fun y => interp_mtree MR In Out x body (k y)).
+Proof.
+  ginit. revert m. gcofix CIH. intros.
+  destruct (observe m) eqn : Heq; symmetry in Heq; apply simpobs in Heq.
+  -  rewrite <- Heq. setoid_rewrite bind_ret_l. apply Reflexive_eqit_gen. auto.
+  - rewrite <- Heq. unfold bind. cbn. rewrite bind_tau. 
+    repeat rewrite interp_mtree_tau. rewrite bind_tau. gstep. constructor.
+    gfinal. left. eapply CIH.
+  - rewrite <- Heq. unfold bind. cbn. rewrite bind_vis.
+    repeat rewrite interp_mtree_vis. destruct (bring_to_front MR x e).
+    destruct x0.
+    + rewrite bind_tau. gstep. constructor. rewrite <- bind_bind. 
+      gfinal. left. eapply CIH.
+    + rewrite bind_vis. gstep. constructor. intros. red.
+      gfinal. left. eapply CIH.
+Qed.
+
+End interp_mtree_bind.
+
+
+Lemma JMeq_comp (A B : Type) (f : A -> B) (g : B -> A) : 
+  f ~= @id B -> g ~= @id A ->
+  forall a, g (f a) = a.
+Proof.
+  intros Hf Hg a. apply JMeq_eq. Set Printing Implicit.
+  (*
+  eapply JMeq_trans with (y:= @id B (@id A a)).
+  2 : reflexivity. Set Printing Implicit. setoid_rewrite Hg.
+  etransitivity.  (id a).
+  Set Printing Implicit. intros a. inv Hf.
+  *)
+Admitted.
+
+Unset Printing Implicit.
+ Section interp_mtree_callm.
+Context (MR : mrec_ctx) (In : Type) (Out : EncodedType In) (x : var (In && Out) MR).
+Context (body : forall i : In, mtree MR (encodes i)).
+Print Assumptions JMeq_comp.
+Lemma interp_mtree_callm (v : In) : interp_mtree MR In Out x body (callm x v) ≈ interp_mtree MR In Out x body (body v).
+Proof.
+  unfold callm.
+  specialize (bring_to_front_call x v) as Hcall1.
+  specialize (call_cont x v) as Hcall2.
+  specialize (bring_to_front_cont x v (projT1 (call x v))) as Hcall3.
+  destruct (call x v). setoid_rewrite bind_trigger.
+  rewrite interp_mtree_vis. cbn in *. 
+  destruct (bring_to_front MR x x0). cbn in *. subst.
+  assert (Hid : forall x, e (e0 x) = x ).
+  { apply JMeq_comp; auto. }
+  cbn in Hid.
+  rewrite tau_eutt. setoid_rewrite interp_mtree_bind.
+  setoid_rewrite interp_mtree_ret. setoid_rewrite <- bind_ret_r at 5.
+  eapply eqit_bind. reflexivity.
+  intros. subst. rewrite Hid. reflexivity.
+Qed.
+
+Context (T1 : Type) (T2 : EncodedType T1) (y : var (T1 && T2) MR).
+Lemma interp_mtree_callm_neq (v : T1) (Hneq : var_neq x y) : 
+                                        interp_mtree MR In Out x body (callm y v) ≈
+                                                     callm (remove_var _ _ _ x y Hneq) v.
+Proof.
+  unfold callm.
+  dependent induction Hneq.
+  - simp call. simp remove_var.
+Admitted.
+(* reason about remove_var, call and bring_to_front *)
+
+End interp_mtree_facts. 
